---
title:  "Operator approach to solving differential equations"
date:   2023-08-01
permalink: posts/odes
---

We will start by solving the following equation:

$$\begin{equation*}
    \frac{dx}{dt} - ax = b
\end{equation*}$$

When solving this equation, a well-known "trick" is usually used. The trick is to multiply the equation by an expression that will make the left side a complete derivative. That expression is called the integrating factor:

$$\begin{align*}

     \frac{dx}{dt} - ax &= b \quad \big{/}\cdot e^{-\int a\,dt} \\

     \left(e^{-\int a\,dt}\right)\frac{dx}{dt} + \left(-ae^{-\int a\,dt}\right)x &= be^{- \int a\,dt}\\

     \frac{d}{dt}\left(xe^{-\int a\,dt}\right) &= be^{-\int a\,dt} \\

     xe^{-\int a\,dt} &= \int be^{-\int a\,dt}\,dt \\

     x &= e^{\int a\,dt}\int be^{-\int a\,dt}\,dt

\end{align*}$$

When $a = \text{const.}$ then the solution reduces to:

$$\begin{equation*}

     x = e^{at}\int be^{-at}\,dt

\end{equation*}$$

## Operators

It turns out that treating differentiation and integration operations as operator applications is very useful. An operator in this sense maps (converts) one function to another. Let's define the following two operators representing the derivative and the indefinite integral, respectively:

$$\begin{align*}

     Dx &\equiv \frac{dx}{dt} \\

     \frac{1}{D}x &\equiv \int x\,dt

\end{align*}$$

Obviously, both operators are linear:

$$\begin{align*}

     D(\alpha x + \alpha y) = \alpha Dx + \beta Dy \\

     \frac{1}{D}(\alpha x + \alpha y) = \alpha \frac{1}{D}x + \beta \frac{1}{D}y

\end{align*}$$

Also, the following symbolic equalities apply:

$$\begin{align*}

     D^{n+1} = D^{n}D \\

     D\frac{1}{D} = 1

\end{align*}$$

The equation \ref{eq:first-order} can be written using the operator as:

$$\begin{align*}

     dx-ax&=b \\

     (D-a)x&=b

\end{align*}$$

previously we could write it symbolically as $b/(D-a)$, having:

$$\begin{equation*}

     \frac{1}{D-a}b = e^{at}\frac{1}{D}e^{-at}\,b

\end{equation*}$$

## Factorization

Differential equations are usually given in the following form:

$$\begin{equation*}

     \frac{d^{n}x}{dt^{n}}+a_{n-1}\frac{d^{n-1}x}{dt^{n-1}} + \cdots + a_ {1}\frac{dx}{dt}+a_{0}x = b

\end{equation*}$$

or written operatorically:

$$\begin{equation*}

     \left ( D^{n}+a_{n-1}D^{n-1} + \cdots + a_{1}D+a_{0}\right )x = b

\end{equation*}$$

The expression in parentheses resembles a polynomial where instead of a variable an operator appears. Since the operator $D$ follows the same rules for addition, multiplication, and exponentiation as the variable, this is a polynomial. Actually, if we wanted to be mathematically rigorous, it is possible to show that such expressions form a ring of polynomials in $D$ over the set of real (or complex) numbers, which allows us to use results from polynomial theory. This means that it is possible to factorize:

$$\begin{equation*}

     (D-\alpha_{1})(D-\alpha_{2})\cdots(D-\alpha_{n})x = b

\end{equation*}$$

With this, we have presented a complex operator consisting of higher-order derivatives as a composition of simple operators consisting at most of the first derivative. It is useful to note that the order of application of the operators in the parentheses is not important. Integrating this equation represents a gradual "removal" of the operator from the left side. The final solution is reached after all simple operators are removed.

$$\begin{align*}(D-\alpha_{2})\cdots(D-\alpha_{n})x &= \frac{1}{D-\alpha_{1}}\,b \\

(D-\alpha_{2})\cdots(D-\alpha_{n})x &= e^{\alpha_{1}t}\frac{1}{D}e^{-\alpha_{1} t}\,b \\

&\cdots \\ x&= e^{\alpha_{n}t}\frac{1}{D}e^{(\alpha_{n-1}-\alpha_{n})t}\cdots e^{ (\alpha_{1}-\alpha_{2})t}\frac{1}{D}e^{-\alpha_{1}t}\,b\end{align*}$$

Therefore, the solution is reached by alternating multiplication and integration. In the general case, when some roots are multiple:

$$\begin{equation*}

     \left [ \prod_{k=1}^{m}(D-\alpha_{k})^{\nu_{k}}\right ]x = b

\end{equation*}$$

the solution is:

$$\begin{equation*}

     x = \left [ \prod_{k=1}^{m}e^{\alpha_{k}t}\frac{1}{D^{\nu_{k}}}e^{-\alpha_{k }t}\right ]b

\end{equation*}$$

Assume that the $x_{j}$ solutions of the equation $(D-\alpha_{j})^{\nu_{j}}x = b$ for $j=1,2,\cdots, m$. Let's observe how the linear combination of these solutions behaves:

$$\begin{align*}\left [ \prod_{k=1}^{m}(D-\alpha_{k})^{\nu_{k}}\right ]\left [ \sum_{j=1} ^{m}\xi_{j}x_{j}\right ] &= b \\

\sum_{j=1}^{m}\xi_{j}\left [ \prod_{k=1}^{m}(D-\alpha_{k})^{\nu_{k}}\right ] x_{j} &= b \\

\sum_{j=1}^{m}\xi_{j}\left [ \prod_{k\neq j}(D-\alpha_{k})^{\nu_{k}}\right ](D- \alpha_{j})^{\nu_{j}}x_{j} &= b \\ \sum_{j=1}^{m}\xi_{j}\left [ \prod_{k\neq j} (D-\alpha_{k})^{\nu_{k}}\right ]b &= b\end{align*}$$

From here it is possible to determine the coefficients $\xi_{j}$:

$$\begin{align*}\sum_{j=1}^{m}\xi_{j}\left [ \prod_{k\neq j}(D-\alpha_{k})^{\nu_{k}} \right ] &= 1\end{align*}$$

Interestingly, the mentioned equation can also be arrived at by breaking it down into partial fractions:

$$\begin{align*}\frac{1}{ \prod_{k=1}^{m}(D-\alpha_{k})^{\nu_{k}}} = \sum_{k=1}^ {m}\frac{\xi_{k}}{(D-\alpha_{k})^{\nu_{k}}}\end{align*}$$
